wip: proofs

Veil/Core/Tools/ModelChecker/ConcreteNew/SearchContext.lean
@@ -7,14 +7,30 @@ namespace Veil.ModelChecker.Concrete
 abbrev SequentialSearchContext (σ κ σₕ : Type) [fp : StateFingerprint σ σₕ] [BEq κ] [Hashable κ] :=
   BaseSearchContext σ κ σₕ × fQueue (QueueItem σₕ σ)
 
--- TODO conjecture: executable things should not become part of this structure
--- (e.g., arguments), otherwise some reference counting will boom?
-structure SequentialSearchContextInvariants {ρ σ κ σₕ : Type}
+variable {ρ σ κ σₕ : Type}
   [fp : StateFingerprint σ σₕ]
   [instBEq : BEq κ] [instHash : Hashable κ]
   {th : ρ}
   (sys : EnumerableTransitionSystem ρ (List ρ) σ (List σ) Int κ (List (κ × ExecutionOutcome Int σ)) th)
   (params : SearchParameters ρ σ)
+
+/-- A sequential search context is stable closed if for any state `u` that
+has been seen and has been fully processed (i.e., not in the queue, not being
+processed), then all its successfully reachable have also been seen. -/
+abbrev SequentialSearchContext.isStableClosed (sctx : SequentialSearchContext σ κ σₕ)
+  -- (Optional) state that is currently being processed
+  (stateInTransit : Option σ) : Prop :=
+  Function.Injective fp.view →
+    (sctx.1.finished = some (.exploredAllReachableStates) ∨ sctx.1.finished = none) →
+      ∀ u ∉ stateInTransit, (fp.view u) ∈ sctx.1.seen →
+        (∀ d : Nat, ⟨fp.view u, u, d⟩ ∉ sctx.2) →
+          ∀ l v, (l, ExecutionOutcome.success v) ∈ sys.tr th u →
+            (fp.view v) ∈ sctx.1.seen
+
+-- TODO conjecture: executable things should not become part of this structure
+-- (e.g., arguments), otherwise some reference counting will boom?
+structure SequentialSearchContextInvariants
+  (stateInTransit : Option σ)
   (sctx : SequentialSearchContext σ κ σₕ)
 extends @SearchContextInvariants ρ σ κ σₕ fp th sys params (· ∈ sctx.2) (· ∈ sctx.1.seen)
 where
@@ -22,11 +38,27 @@ where
   -- being a special case
   init_states_included : ∀ s ∈ sys.initStates, (fp.view s) ∈ sctx.1.seen
   terminate_empty_queue : sctx.1.finished = some (.exploredAllReachableStates) → sctx.2.isEmpty
-  stable_closed :  Function.Injective fp.view →
-    (sctx.1.finished = some (.exploredAllReachableStates) ∨ sctx.1.finished = none) →
-      ∀ u : σ, (fp.view u) ∈ sctx.1.seen →
-        (∀ d : Nat, ⟨fp.view u, u, d⟩ ∉ sctx.2) →
-          ∀ l v, (l, ExecutionOutcome.success v) ∈ sys.tr th u →
-          (fp.view v) ∈ sctx.1.seen
+  stable_closed : sctx.isStableClosed sys stateInTransit
+
+abbrev LawfulSequentialSearchContext (stateInTransit : Option σ := .none) : Type :=
+  Subtype (α := SequentialSearchContext σ κ σₕ) (SequentialSearchContextInvariants sys params stateInTransit)
+
+/-- When finishing processing a state, we move from having that state `curr`
+in transit to having no state in transit, provided that all successfully
+reachable neighbors of `curr` in transit have been seen. -/
+theorem SequentialSearchContextInvariants.finish_stateInTransit
+  {sctx : SequentialSearchContext σ κ σₕ}
+  {curr : σ}
+  (sctx_invs : SequentialSearchContextInvariants sys params (.some curr) sctx)
+  (h_neighbors_seen : ∀ l v, (l, ExecutionOutcome.success v) ∈ sys.tr th curr →
+    (fp.view v) ∈ sctx.1.seen) :
+  SequentialSearchContextInvariants sys params .none sctx := by
+  rcases sctx with ⟨ctx, sq⟩ ; rcases sctx_invs with ⟨h1, h2, h3, h_closed⟩ ; dsimp only at *
+  constructor <;> try assumption
+  simp [SequentialSearchContext.isStableClosed] at h_closed ⊢
+  intro ha hb u hc hd l v hin
+  by_cases heq : curr = u
+  on_goal 2=> grind
+  subst u ; eapply h_neighbors_seen ; assumption
 
 end Veil.ModelChecker.Concrete
